feat: Term.rename

Cslib/Languages/LambdaCalculus/Named/Coc/Basic.lean
@@ -39,6 +39,23 @@ inductive Term (Var : Type u) : Type u
   | type : Term Var
 deriving DecidableEq
 
+namespace Term
+
+/-- Renaming, or variable substitution. `m.rename x y` renames `x` into `y` in `m`. -/
+def rename [DecidableEq Var] (m : Term Var) (x : Var) (y : Var) : Term Var := match m with
+  | .var z => if z = x then .var y else .var z
+  | .app f a => .app (f.rename x y) (a.rename x y)
+  | .lam v t b => .lam v (t.rename x y) (b.rename x y)
+  | .pi v t b => .pi v (t.rename x y) (b.rename x y)
+  | .type => .type
+
+/-- Renaming preserves size. -/
+theorem rename.eq_sizeOf {m : Term Var} {x y : Var} [DecidableEq Var] :
+    sizeOf (m.rename x y) = sizeOf m := by
+  induction m <;> simp_all [Term.rename] ; split <;> simp_all
+
+end Term
+
 end LambdaCalculus.Named.Coc
 
 end Cslib
